IMP-_To_SAS+/IMP_Minus_To_SAS_Plus.thy
@@ -7,14 +7,17 @@ theory IMP_Minus_To_SAS_Plus
     "IMP--_To_SAS++/IMP_Minus_Minus_To_SAS_Plus_Plus_Correctness"
     "SAS++_To_SAS+/SAS_Plus_Plus_To_SAS_Plus"
     "IMP_Minus_Max_Constant"
+    "HOL-Library.Discrete"
 begin
 
 type_synonym SAS_problem = "(IMP_Minus_Minus_To_SAS_Plus_Plus_State_Translations.variable, 
   IMP_Minus_Minus_To_SAS_Plus_Plus_State_Translations.domain_element) problem" 
 
-fun bit_length::"nat \<Rightarrow> nat" where
-"bit_length  0 = 0" | 
-"bit_length  n = 1 + bit_length (n div 2) "
+definition bit_length where "bit_length x \<equiv>  Discrete.log x + 1"
+
+lemma le_two_to_the_bit_length_intro: "x \<le> y \<Longrightarrow> x \<le> 2 ^ (bit_length y)"
+  apply(auto simp: bit_length_def)
+  by (metis leD log_exp2_gt max.strict_coboundedI2 max_def)
 
 definition max_input_bits:: "IMP_Minus_com \<Rightarrow> (vname \<rightharpoonup> nat) \<Rightarrow> nat \<Rightarrow> nat" where
 "max_input_bits c I r = 
@@ -23,15 +26,129 @@ definition max_input_bits:: "IMP_Minus_com \<Rightarrow> (vname \<rightharpoonup
 definition IMP_Minus_to_SAS_Plus:: "IMP_Minus_com \<Rightarrow> (vname \<rightharpoonup> nat) \<Rightarrow> nat \<Rightarrow> (vname \<rightharpoonup> nat) 
   \<Rightarrow>  nat \<Rightarrow> SAS_problem" where
 "IMP_Minus_to_SAS_Plus c I r G t = (let 
-  n = max_input_bits c I r ;
-  I' = (\<lambda>x. Some (Num x)) \<circ>\<^sub>m I ;
-  G' = (\<lambda>x. Some (Num x)) \<circ>\<^sub>m G in 
-  SAS_Plus_Plus_To_SAS_Plus (imp_minus_minus_to_sas_plus (IMP_Minus_To_IMP_Minus_Minus c n) I' G' t))"
+  n = t + max_input_bits c I r + 1;
+  t' = (100 * n * (t - 1) + 51) in
+  (let c' = IMP_Minus_To_IMP_Minus_Minus c n in
+  (let I' = ((\<lambda>x. Some (Num x)) \<circ>\<^sub>m (IMP_Minus_State_To_IMP_Minus_Minus_partial I n)) 
+    |` (set (enumerate_variables c')) ;
+  G' = ((\<lambda>x. Some (Num x)) \<circ>\<^sub>m (IMP_Minus_State_To_IMP_Minus_Minus_partial G n))
+    |` (set (enumerate_variables c')) in 
+  SAS_Plus_Plus_To_SAS_Plus (imp_minus_minus_to_sas_plus c' I' G' t'))))"
+
+lemma le_mul_intro: "0 < b \<Longrightarrow> a \<le> b \<Longrightarrow> (1 :: nat) < c \<Longrightarrow> a < c * b" 
+  by (metis One_nat_def dual_order.strict_trans le_neq_implies_less n_less_m_mult_n)
 
 lemma IMP_Minus_to_SAS_Plus_correctness:
-  assumes "finite (ran I)"
-    "\<forall>s. \<exists>s2. \<exists>t' \<le> t. (c, s1) \<Rightarrow>\<^bsup>t'\<^esup> s2"
-  shows  "(\<exists>s1 s2 t'. I \<subseteq>\<^sub>m Some \<circ> s1 \<and> G  \<subseteq>\<^sub>m Some \<circ> s2 \<and> (c, s1) \<Rightarrow>\<^bsup>t'\<^esup> s2)
-    \<longleftrightarrow> (\<exists>plan. length plan \<le> 100 * (max_input_bits c I r) * (t - 1) + 100 + 
+  assumes
+    "I \<subseteq>\<^sub>m Some \<circ> s1" 
+    "finite (range s1)" 
+    "Max (range s1) < r"
+    "G \<subseteq>\<^sub>m Some \<circ> s2"
+    "(c, s1) \<Rightarrow>\<^bsup>t\<^esup> s2"
+  shows "\<exists>plan. length plan \<le> 100 * (max_input_bits c I r + t + 1) * (t - 1) 
+      + (max_input_bits c I r + t + 1 + 1) * (num_variables c + 2) + 52
+      \<and> is_serial_solution_for_problem (IMP_Minus_to_SAS_Plus c I r G t) plan"
+proof -
+  let ?n = "t + max_input_bits c I r + 1"
+  let ?c' = "IMP_Minus_To_IMP_Minus_Minus c ?n"
+  let ?s1' = "IMP_Minus_State_To_IMP_Minus_Minus s1 ?n"
+  let ?s2' = "IMP_Minus_State_To_IMP_Minus_Minus s2 ?n"
+  let ?I = "((\<lambda>x. Some (Num x)) \<circ>\<^sub>m (IMP_Minus_State_To_IMP_Minus_Minus_partial I ?n))
+    |` (set (enumerate_variables ?c'))"
+  let ?G = "((\<lambda>x. Some (Num x)) \<circ>\<^sub>m (IMP_Minus_State_To_IMP_Minus_Minus_partial G ?n))
+    |` (set (enumerate_variables ?c'))"
+  let ?t = "100 * ?n * (t - 1) + 51"
+  let ?sas_plus_plus_problem 
+    = "imp_minus_minus_to_sas_plus (IMP_Minus_To_IMP_Minus_Minus c ?n) ?I ?G ?t"
+
+  have "t_small_step_fun (100 * ?n * (t - 1) + 50) 
+      (IMP_Minus_To_IMP_Minus_Minus c ?n, IMP_Minus_State_To_IMP_Minus_Minus s1 ?n)
+     = (SKIP, IMP_Minus_State_To_IMP_Minus_Minus s2 ?n)" 
+    apply - apply(rule IMP_Minus_To_IMP_Minus_Minus)
+    using assms apply(auto simp: max.strict_coboundedI1 max.strict_coboundedI2 max_input_bits_def 
+        power_add intro!: le_mul_intro le_two_to_the_bit_length_intro) 
+    by (metis less_imp_le_nat max.coboundedI1 max.commute)
+
+  then obtain t' where t'_def: "t' \<le> 100 * ?n * (t - 1) + 50" "(?c', ?s1') \<rightarrow>\<^bsup>t'\<^esup> (SKIP, ?s2')" 
+    using t_small_step_fun_t_small_step_equivalence by auto
+
+  let ?s1'' = "canonical_\<omega>_state (t' + 1) ?c' ?s1'"
+  have "\<exists>s2''. ((?c', ?s1'') \<rightarrow>\<^bsub>?t\<^esub>\<^bsup>t'\<^esup> (SKIP, s2'')) 
+    \<and> dom s2'' = set (enumerate_variables ?c') 
+    \<and> \<omega>_equivalent ((t' + 1) - t' * IMP_Minus_Minus_Domains.max_constant ?c') ?s2' s2''"
+    using  t'_def c_in_all_subprograms_c  IMP_Minus_To_IMP_Minus_Minus_max_constant
+    apply(auto simp: canonical_\<omega>_state_\<omega>_equivalent le_imp_less_Suc 
+        intro!: small_step_omega_equivalence)
+    by(auto simp: canonical_\<omega>_state_def split: if_splits)
+  then obtain s2'' where s2''_def: "((?c', ?s1'') \<rightarrow>\<^bsub>?t\<^esub>\<^bsup>t'\<^esup> (SKIP, s2'')) "
+    "dom s2'' = set (enumerate_variables ?c')"
+    "\<omega>_equivalent ((t' + 1) - t' * IMP_Minus_Minus_Domains.max_constant ?c') ?s2' s2''" by blast
+  hence "\<omega>_equivalent 1 ?s2' s2''" 
+    apply - apply(rule \<omega>_equivalent_increasing') 
+    using IMP_Minus_To_IMP_Minus_Minus_max_constant apply auto
+    by (metis Nat.le_add_diff One_nat_def add.commute nat_mult_1_right nat_mult_le_cancel_disj 
+        plus_1_eq_Suc)
+  hence "?G v = Some y \<Longrightarrow> s2'' v = Some y" for v y
+  proof-
+    assume "?G v = Some y"
+    then obtain y' where "y = Num y'" by(auto simp: map_comp_Some_iff)
+    hence "?s2' v = y'" using \<open>?G v = Some y\<close> \<open>G \<subseteq>\<^sub>m Some \<circ> s2\<close> 
+      by(auto simp: map_le_def map_comp_Some_iff IMP_Minus_State_To_IMP_Minus_Minus_partial_def 
+        IMP_Minus_State_To_IMP_Minus_Minus_def dom_def var_to_var_bit_eq_Some_iff
+          split: option.splits if_splits)+
+    moreover have "v \<in> dom s2''" using \<open>?G v = Some y\<close> \<open>dom s2'' = set (enumerate_variables ?c')\<close>
+      by auto
+    ultimately show "s2'' v = Some y" using \<open>\<omega>_equivalent 1 ?s2' s2''\<close> \<open>y = Num y'\<close>
+      by(auto simp: \<omega>_equivalent_def less_nth_bit_iff
+            dom_def var_to_var_bit_eq_Some_iff IMP_Minus_State_To_IMP_Minus_Minus_bounded
+            split: option.splits if_splits)
+  qed
+  hence "?G \<subseteq>\<^sub>m s2''" by (auto simp: map_le_def)
+
+  let ?ss1'' = "imp_minus_state_to_sas_plus (?c', ?s1'')" 
+  let ?ss2'' = "imp_minus_state_to_sas_plus (SKIP, s2'')" 
+  have "max 1 (IMP_Minus_Minus_Domains.max_constant ?c') = 1" 
+    using IMP_Minus_To_IMP_Minus_Minus_max_constant by (simp add: max.absorb1)
+  hence "\<exists>plan. is_serial_solution_for_problem_sas_plus_plus ?sas_plus_plus_problem plan
+     \<and> length plan = t'"
+    using s2''_def t'_def 
+    apply(auto simp: canonical_\<omega>_state_def IMP_Minus_State_To_IMP_Minus_Minus_def 
+      IMP_Minus_To_IMP_Minus_Minus_variables split: if_splits option.splits 
+      intro!: \<omega>_imp_minus_minus_to_sas_plus_plus[where ?is1.0="?s1''"] nth_bit_le_intro)
+     using \<open>I \<subseteq>\<^sub>m Some \<circ> s1\<close> 
+      apply(fastforce simp: map_le_def canonical_\<omega>_state_eq_Some_iff 
+        IMP_Minus_State_To_IMP_Minus_Minus_def
+        map_comp_def IMP_Minus_State_To_IMP_Minus_Minus_partial_def dom_def nth_bit_le_intro
+        IMP_Minus_To_IMP_Minus_Minus_variables
+        elim!: set_mp[OF IMP_Minus_To_IMP_Minus_Minus_variables]
+        split!: option.splits if_splits)
+     using \<open>?G \<subseteq>\<^sub>m s2''\<close> by auto
+   then obtain plan where plan_def: 
+     "is_serial_solution_for_problem_sas_plus_plus ?sas_plus_plus_problem plan"
+      "length plan = t'" by blast
+
+   hence "\<exists>prefix. length prefix \<le> length ((?sas_plus_plus_problem)\<^sub>\<V>\<^sub>+) + 1 
+    \<and> is_serial_solution_for_problem (SAS_Plus_Plus_To_SAS_Plus ?sas_plus_plus_problem) 
+        (prefix @ (map SAS_Plus_Plus_Operator_To_SAS_Plus_Operator plan))"
+     apply -
+     apply(rule SAS_Plus_Plus_To_SAS_Plus)
+     apply(rule imp_minus_minus_to_sas_plus_valid)
+     by(auto simp: IMP_Minus_State_To_IMP_Minus_Minus_partial_def map_comp_def nth_bit_le_intro
+         split: option.splits)
+   then obtain prefix where prefix_def: "length prefix \<le> length ((?sas_plus_plus_problem)\<^sub>\<V>\<^sub>+) + 1 
+    \<and> is_serial_solution_for_problem (SAS_Plus_Plus_To_SAS_Plus ?sas_plus_plus_problem) 
+        (prefix @ (map SAS_Plus_Plus_Operator_To_SAS_Plus_Operator plan))" by blast
+   let ?plan' = "prefix @ (map SAS_Plus_Plus_Operator_To_SAS_Plus_Operator plan)"
+   have "length ((?sas_plus_plus_problem)\<^sub>\<V>\<^sub>+) \<le> (?n + 1) * (num_variables c + 2) + 1" using 
+     IMP_Minus_To_IMP_Minus_Minus_variables_length[where ?c=c 
+         and ?n="(Suc (t + max_input_bits c I r))"] 
+     by(auto simp: imp_minus_minus_to_sas_plus_def Let_def)
+   hence "length prefix \<le> (?n + 1) * (num_variables c + 2) + 2" using prefix_def by simp
+   hence "length ?plan' \<le> 100 * ?n * (t - 1) + (?n + 1) * (num_variables c + 2) + 52
+      \<and> is_serial_solution_for_problem (IMP_Minus_to_SAS_Plus c I r G t) ?plan'"
+     using plan_def prefix_def t'_def by(auto simp: IMP_Minus_to_SAS_Plus_def Let_def)
+   thus ?thesis by (metis add.commute)
+ qed
+    
 
 end
